src/MinimalND.v
@@ -1,0 +1,139 @@
+Require Import Coq.ZArith.BinInt.
+Require Import riscv.util.BitWidths.
+Require Import riscv.util.Monads.
+Require Import riscv.Decode.
+Require Import riscv.Memory. (* should go before Program because both define loadByte etc *)
+Require Import riscv.Program.
+Require Import riscv.Execute.
+Require Import riscv.util.PowerFunc.
+Require Import riscv.Utility.
+Require Import Coq.Lists.List. Import ListNotations.
+Require Import riscv.Minimal.
+
+Section Riscv.
+
+  Context {t: Set}.
+
+  Context {MW: MachineWidth t}.
+
+  Context {Mem: Set}.
+
+  Context {MemIsMem: Memory Mem t}.
+
+  Context {RF: Type}.
+  Context {RFI: RegisterFile RF Register t}.
+
+  (* MMIO trace *)
+  Inductive LogEvent :=
+  | EvInput(addr: Z)(v: word 32)
+  | EvOutput(addr: Z)(v: word 32).
+
+  Definition Log := list LogEvent.
+
+  Record RiscvMachineL := mkRiscvMachineL {
+    machine: @RiscvMachine t Mem RF;
+    log: Log;
+  }.
+
+  Definition with_machine m ml := mkRiscvMachineL m ml.(log).
+  Definition with_log l ml := mkRiscvMachineL ml.(machine) l.
+
+(*
+  Definition liftL0{B: Type}(f: OStateND (@RiscvMachine t Mem RF) B):  OStateND RiscvMachineL B (*:=
+    fun s => let (ob, ma) := f s.(machine) in (ob, with_machine ma s).*)
+. Admitted.
+
+  Definition liftL1{A B: Type}(f: A -> OStateND (@RiscvMachine t Mem RF) B): A -> OStateND RiscvMachineL B. (* :=
+    fun a s => let (ob, ma) := f a s.(machine) in (ob, with_machine ma s).*) Admitted.
+
+  Definition liftL2{A1 A2 B: Type}(f: A1 -> A2 -> OStateND (@RiscvMachine t Mem RF) B):
+    A1 -> A2 -> OStateND RiscvMachineL B. (*  :=
+    fun a1 a2 s => let (ob, ma) := f a1 a2 s.(machine) in (ob, with_machine ma s). *)
+  Admitted.
+*)
+  Definition liftL0{B: Type}(f: OState (@RiscvMachine t Mem RF) B):  OStateND RiscvMachineL B (*:=
+    fun s => let (ob, ma) := f s.(machine) in (ob, with_machine ma s).*)
+. Admitted.
+
+  Definition liftL1{A B: Type}(f: A -> OState (@RiscvMachine t Mem RF) B): A -> OStateND RiscvMachineL B. (* :=
+    fun a s => let (ob, ma) := f a s.(machine) in (ob, with_machine ma s).*) Admitted.
+
+  Definition liftL2{A1 A2 B: Type}(f: A1 -> A2 -> OState (@RiscvMachine t Mem RF) B):
+    A1 -> A2 -> OStateND RiscvMachineL B. (*  :=
+    fun a1 a2 s => let (ob, ma) := f a1 a2 s.(machine) in (ob, with_machine ma s). *)
+  Admitted.
+
+  Definition TODO{A: Type}: A. Admitted.
+
+  Definition get: OStateND RiscvMachineL RiscvMachineL.
+    intro s. intro set.
+    apply (forall mach ans, set mach ans <-> ans = Some mach /\ mach = s).
+  Defined.
+
+  Definition put(s: RiscvMachineL): OStateND RiscvMachineL unit.
+    refine (fun initial set => forall mach ans, set mach ans <-> mach = s /\ ans = Some tt).
+  Defined.
+
+  Definition failure{A}: OStateND RiscvMachineL A := fun s outcomes => False.
+
+  Definition success{A}(set: RiscvMachineL -> option A -> Prop): OStateND RiscvMachineL A.
+    refine (fun initial set' => forall mach ans, set' mach ans <-> set mach ans).
+  Defined.
+
+  Definition deterministic{S A}(m: S)(ans: option A): S -> option A -> Prop :=
+    fun s ans' => s = m /\ ans = ans'. (* todo * instead of curry and jus eq *)
+
+  Definition arbitrary(A: Type): OStateND RiscvMachineL A.
+    refine (s <- get; success _).
+    refine (fun s' oa => s = s' /\ exists a, oa = Some a).
+  Defined.
+
+  Definition answer{A: Type}(ans: A): OStateND RiscvMachineL A :=
+    s <- get; success (deterministic s (Some ans)).
+
+  (* recoverable (through option) *)
+  Definition throw{A}: OStateND RiscvMachineL A :=
+    s <- get; success (deterministic s None).
+
+  Definition logEvent(e: LogEvent): OStateND RiscvMachineL unit :=
+    m <- get; put (with_log (e :: m.(log)) m).
+
+  Definition isMMIOAddr(a: t): bool. Admitted.
+
+  Instance IsRiscvMachineL: RiscvProgram (OStateND RiscvMachineL) t :=  {|
+      getRegister := liftL1 getRegister;
+      setRegister := liftL2 setRegister;
+      getPC := liftL0 getPC;
+      setPC := liftL1 setPC;
+      loadByte   := liftL1 loadByte;
+      loadHalf   := liftL1 loadHalf;
+      loadWord a := if isMMIOAddr a
+                    then
+                      inp <- arbitrary (word 32);
+                      logEvent (EvInput (regToZ_unsigned a) inp);; answer inp
+                    else liftL1 loadWord a;
+      loadDouble := liftL1 loadDouble;
+      storeByte   := liftL2 storeByte;
+      storeHalf   := liftL2 storeHalf;
+      storeWord a v := TODO;
+      storeDouble := liftL2 storeDouble;
+      step := liftL0 step;
+      getCSRField_MTVecBase := liftL0 getCSRField_MTVecBase;
+      endCycle A := TODO;
+  |}.
+(*
+  - refine (if isMMIOAddr a then _ else _).
+    { refine (inp <- arbitrary (word 32); _).
+      refine (logEvent (EvInput (regToZ_unsigned a) inp);; answer inp).
+    }
+    {
+      exact (liftL1 loadWord a).
+    }
+  Defined.
+*)
+  Definition putProgram(prog: list (word 32))(addr: t)(ma: RiscvMachineL): RiscvMachineL :=
+    with_machine (putProgram prog addr ma.(machine)) ma.
+
+End Riscv.
+
+Existing Instance IsRiscvMachineL. (* needed because it was defined inside a Section *)
